Denotational-Props.thy
@@ -1,0 +1,470 @@
+theory "Denotational-Props"
+  imports "Denotational"
+begin
+
+lemma ESem_cont_induct_lemma:
+  "subpcpo (compatible_with_exp e d) \<and> cont_on (compatible_with_exp e d) (\<lambda>\<rho>'. \<lbrakk> e \<rbrakk>\<^bsub>\<rho>'\<^esub>)" and True
+proof(nominal_induct e and rule:exp_assn.strong_induct)
+  
+oops
+(*
+lemma ESem_cont':"Y0 = Y 0 \<Longrightarrow> chain Y \<Longrightarrow> range (\<lambda>i. \<lbrakk> e \<rbrakk>\<^bsub>Y i\<^esub>) <<| \<lbrakk> e \<rbrakk>\<^bsub>(\<Squnion> i. Y i)\<^esub> " and True
+proof(nominal_induct e and avoiding: Y0  arbitrary: Y rule:exp_assn.strong_induct)
+case (Lam x e Y0 Y)
+  have [simp]: "\<And> i. fdom (Y i) = fdom (Lub Y)"
+    by (metis chain_fdom `chain Y`)
+  have [simp]:"\<And> i. atom x \<sharp> Y i" and [simp]:"atom x \<sharp> Lub Y"  using Lam.hyps(1) Lam.prems(1)
+    unfolding sharp_Env by auto
+  have "cont (ESem e)" using Lam.hyps(2) by (rule contI, auto)
+  have  "cont (\<lambda> \<rho>. Fn\<cdot>(\<Lambda> v. \<lbrakk> e \<rbrakk>\<^bsub>\<rho>(x f\<mapsto> v)\<^esub>))"
+    by (intro cont2cont cont_compose[OF `cont (ESem e)`])
+  from contE[OF this, OF Lam.prems(2)]
+  show ?case
+    by simp
+next
+case (App e v Y0 Y)
+  have "cont (ESem e)" using App.hyps(1) by (rule contI, auto)
+  thus ?case
+    by (auto intro:contE[OF _ App.prems(2)])
+next
+case (Var v Y0 Y)
+  have "cont (\<lambda> \<rho>. ESem (Var v) \<rho>)" by auto
+  thus ?case
+    by (rule contE[OF _ Var.prems(2)])    
+next
+case (Let as e Y0 Y)
+  have [simp]: "\<And> i. fdom (Y i) = fdom (Lub Y)"
+    by (metis chain_fdom `chain Y`)
+  have [simp]:"\<And> i. set (bn as) \<sharp>* Y i" and [simp]: "set (bn as) \<sharp>* Lub Y"  using Let.hyps(1) Let.prems(1)
+    unfolding sharp_star_Env by auto
+  have "cont (ESem e)" using Let.hyps(3) by (rule contI, auto)
+  show ?case
+    by (simp, intro contE[OF _ Let.prems(2)] cont2cont cont_compose[OF `cont (ESem e)`])
+qed simp
+
+lemma ESem_cont: "cont (ESem e)"  using ESem_cont'[OF refl] by (rule contI)
+
+lemmas ESem_cont2cont[simp,cont2cont] = cont_compose[OF ESem_cont]
+*)
+
+definition HSem ("\<lbrace>_\<rbrace>_"  [60,60] 60) where "\<lbrace>\<Gamma>\<rbrace>\<rho> = heapExtendMeet \<rho> \<Gamma> ESem"
+
+lemma Esem_simps4[simp]: "set (bn as) \<sharp>* \<rho> \<Longrightarrow> \<lbrakk> Terms.Let as body \<rbrakk>\<^bsub>\<rho>\<^esub> = \<lbrakk> body \<rbrakk>\<^bsub>\<lbrace>asToHeap as \<rbrace>\<rho>\<^esub>"
+  by (simp add: HSem_def)
+(*
+lemma HSem_def': "\<lbrace>\<Gamma>\<rbrace>\<rho> = fmap_meet \<rho> (fix1 (fmap_bottom (fst ` set \<Gamma>)) (\<Lambda> \<rho>'. heapToEnv \<Gamma> (\<lambda>e. \<lbrakk>e\<rbrakk>\<^bsub>fmap_meet \<rho> \<rho>'\<^esub>))) "
+  unfolding HSem_def heapExtendMeet_def by simp
+*)
+declare ESem.simps(4)[simp del]
+
+(*
+lemma HSem_cont2: "cont (\<lambda>y. HSem \<Gamma> y)"
+  unfolding HSem_def' by auto
+
+lemmas HSem_cont2cont[cont2cont,simp] = cont_compose[OF HSem_cont2]
+*)
+
+lemma HSem_eqvt[eqvt]: "\<pi> \<bullet> (\<lbrace>\<Gamma>\<rbrace>\<rho>) = \<lbrace>\<pi> \<bullet> \<Gamma>\<rbrace>(\<pi> \<bullet> \<rho>)"
+  unfolding HSem_def
+  by (perm_simp, rule)
+
+lemma HSem_Nil[simp]: "\<lbrace>[]\<rbrace>\<rho> = \<rho>"
+  unfolding HSem_def heapExtendMeet_def heapToEnv.simps by auto
+
+(*
+lemma HSem_def'': "\<lbrace>\<Gamma>\<rbrace>\<rho> = fix1 (fmap_update \<rho> (fmap_bottom (fst ` set \<Gamma>))) (\<Lambda> \<rho>'. fmap_update \<rho> (heapToEnv \<Gamma> (\<lambda>e. \<lbrakk>e\<rbrakk>\<^bsub>\<rho>'\<^esub>)))"
+  unfolding HSem_def'
+  apply (rule parallel_fix1_ind)
+  by (auto intro: cont2monofunE[OF fmap_update_cont2])
+
+
+lemma HSem_def''': "\<lbrace>\<Gamma>\<rbrace>\<rho> = fix1 ((fmap_bottom (fdom \<rho> \<union> fst ` set \<Gamma>))) (\<Lambda> \<rho>'. fmap_update \<rho> (heapToEnv \<Gamma> (\<lambda>e. \<lbrakk>e\<rbrakk>\<^bsub>\<rho>'\<^esub>)))"
+  unfolding HSem_def''
+  apply (rule fix1_alt_start[symmetric])
+  apply auto[1]
+  apply simp
+  apply (rule cont2monofunE[OF fmap_update_cont2])
+  apply simp
+  done
+
+lemma [simp]:"fdom (\<lbrace>\<Gamma>\<rbrace>\<rho>) = fdom \<rho> \<union> fst ` set \<Gamma>"
+  unfolding HSem_def' by auto
+
+lemma [simp]: "x \<notin> fst ` set \<Gamma> \<Longrightarrow> lookup (\<lbrace>\<Gamma>\<rbrace>\<rho>) x = lookup \<rho> x"
+  unfolding HSem_def' by auto
+
+
+lemma fdom_fmap_restr_Hsem[simp]: "fdom (fmap_restr (fst ` set \<Gamma>) (\<lbrace>\<Gamma>\<rbrace>\<rho>')) = fst ` set \<Gamma>"
+  by auto
+
+*)
+
+
+
+lemma fmap_upd_fix1: 
+  assumes above: "x0 \<sqsubseteq> F\<cdot>x0"
+    and permute: "\<And>z. (F\<cdot>z)(x f\<mapsto> y) = F\<cdot>(z(x f\<mapsto> y))"
+    shows "(fix1 x0 F) (x f\<mapsto> y) = fix1 (x0 (x f\<mapsto> y)) (\<Lambda> z. (F\<cdot>z)(x f\<mapsto> y))"
+  apply (rule parallel_fix1_ind)
+  apply auto[1]
+  apply (rule above)
+  apply simp
+  apply (subst permute[symmetric])
+  apply simp
+  apply (rule cont2monofunE[OF fmap_upd_cont[OF cont_id cont_const]])
+  apply (rule above)
+  apply (rule refl)
+  apply simp
+  apply (subst (1 2) permute)
+  apply (rule cfun_arg_cong[of _ _ F])
+  apply (drule sym)
+  apply simp
+  done
+
+lemma fmap_update_fix1: 
+  assumes above: "x0 \<sqsubseteq> F\<cdot>x0"
+    and permute: "\<And>z. fmap_update \<rho> (F\<cdot>z) = F \<cdot> (fmap_update \<rho> z)"
+    shows "fmap_update \<rho> (fix1 x0 F) = fix1 (fmap_update \<rho> x0) (\<Lambda> z. fmap_update \<rho> (F\<cdot>z))"
+  apply (rule parallel_fix1_ind)
+  apply auto[1]
+  apply (rule above)
+  apply simp
+  apply (subst permute[symmetric])
+  apply simp
+  apply (rule cont2monofunE[OF fmap_update_cont2cont[OF cont_const cont_id]])
+  apply (rule above)
+  apply (rule refl)
+  apply simp
+  apply (subst (1 2) permute)
+  apply (rule cfun_arg_cong[of _ _ F])
+  apply (drule sym)
+  apply simp
+  done
+
+
+lemma tmp:"fmap_update \<rho> ((iterate i F) \<cdot> x) = (iterate i (\<Lambda> x. fmap_update \<rho> (F \<cdot> x))) \<cdot> (fmap_update \<rho> x)" sorry
+
+lemmas tmp2 =  cont2contlubE[of "\<lambda> y. (iterate i (\<Lambda> \<rho>'. fmap_update \<rho> ((y)(x f\<mapsto> G \<rho>'))))\<cdot>x0", standard]
+thm tmp2
+
+
+lemma  fmap_update_belowI:
+  assumes "fdom x \<union> fdom y = fdom z"
+  and "\<And> a. a \<in> fdom y \<Longrightarrow> the (lookup y a) \<sqsubseteq> the (lookup z a)"
+  and "\<And> a. a \<in> fdom x \<Longrightarrow> a \<notin> fdom y \<Longrightarrow> the (lookup x a) \<sqsubseteq> the (lookup z a)"
+  shows  "fmap_update x y \<sqsubseteq> z"
+  using assms 
+  apply -
+  apply (rule fmap_belowI)
+  apply auto[1]
+  by (metis fdomIff lookup_fmap_update1 lookup_fmap_update2 the.simps)
+
+(*
+lemma HSem_unroll: "\<lbrace>\<Gamma>\<rbrace>\<rho> = fmap_update \<rho> (heapToEnv \<Gamma> (\<lambda> e. \<lbrakk>e\<rbrakk>\<^bsub>\<lbrace>\<Gamma>\<rbrace>\<rho>\<^esub>))"
+  apply(subst (1 2) HSem_def''')
+  apply(subst fix_eq)
+  apply auto
+  done
+*)
+
+(*
+lemma iterative_HSem:
+  assumes "x \<notin> fst ` set \<Gamma>"
+  shows "\<lbrace>(x,e) # \<Gamma>\<rbrace>\<rho> = fix1 (fmap_bottom (fdom \<rho> \<union> fst ` set ((x,e) # \<Gamma>))) (\<Lambda> \<rho>'. fmap_update \<rho> ((fmap_restr (fst ` set \<Gamma>) (\<lbrace>\<Gamma>\<rbrace>\<rho>'))(x f\<mapsto> \<lbrakk>e\<rbrakk>\<^bsub>\<rho>'\<^esub>)))" (is "_ = fix1 _ ?R")
+apply (subst HSem_def''')
+proof(rule below_antisym)
+  let "fix1 ?x0 ?L" = "fix1 (fmap_bottom (fdom \<rho> \<union> fst ` set ((x, e) # \<Gamma>))) (\<Lambda> \<rho>'. fmap_update \<rho> (heapToEnv ((x, e) # \<Gamma>) (\<lambda>e. \<lbrakk> e \<rbrakk>\<^bsub>\<rho>'\<^esub>)))"
+
+  have "?x0 \<sqsubseteq> ?L\<cdot>?x0"
+    by (auto intro: cont2monofunE[OF fmap_update_cont2])
+  (* have "?x0 \<sqsubseteq> ?R\<cdot>?x0" 
+    apply (rule fmap_bottom_below)
+    by (auto)*)
+  have "?x0 \<sqsubseteq> ?R\<cdot>?x0" 
+    by simp
+
+{
+  show "fix1 ?x0 ?L \<sqsubseteq> fix1 ?x ?R"
+  proof(rule fix_least_below[OF `?x0 \<sqsubseteq> ?L\<cdot>?x0`])
+    let "?y" = "fix1 ?x ?R"
+    show  "?x0 \<sqsubseteq> ?y"
+      apply (rule start_below_fix1)
+      apply (rule fmap_bottom_below)
+      apply auto
+      done
+
+    have large_fdom[simp]: "fdom ((fmap_restr (fst ` set \<Gamma>) (\<lbrace>\<Gamma>\<rbrace>?y))(x f\<mapsto> \<lbrakk> e \<rbrakk>\<^bsub>?y\<^esub>)) = insert x (fst ` set \<Gamma>)"
+      by simp
+
+    have "?L\<cdot>?y \<sqsubseteq> ?R\<cdot>?y"
+    proof (rule fmap_belowI')
+      show "fdom (?L\<cdot>?y) = fdom (?R\<cdot>?y)" using fmap_below_dom[OF `?x0 \<sqsubseteq> ?y`] by auto
+    next
+      fix x'
+      assume "x' \<in> fdom (?L\<cdot>?y)" and "x' \<in> fdom (?R\<cdot>?y)"
+      show "the (lookup (?L\<cdot>?y) x') \<sqsubseteq> the (lookup (?R\<cdot>?y) x')"
+      proof (cases "x' = x")
+        case True thus ?thesis by auto
+      next
+        case False note F1 = this thus ?thesis
+        proof (cases "x' \<in> fdom (heapToEnv ((x, e) # \<Gamma>) (\<lambda>e. \<lbrakk> e \<rbrakk>\<^bsub>?y\<^esub>))")
+        case True
+          moreover
+          hence "x' \<in> fdom ((fmap_restr (fst ` set \<Gamma>) (\<lbrace>\<Gamma>\<rbrace>?y))(x f\<mapsto> \<lbrakk> e \<rbrakk>\<^bsub>?y\<^esub>))" by auto
+          moreover
+          hence "x' \<in> fst ` set \<Gamma>" using F1 by auto
+          moreover
+          {
+            (*
+            have "the (lookup (heapToEnv \<Gamma> (\<lambda>e. \<lbrakk> e \<rbrakk>\<^bsub>?y\<^esub>)) x')  \<sqsubseteq>
+              the (lookup (heapToEnv \<Gamma> (\<lambda>e. \<lbrakk> e \<rbrakk>\<^bsub>fmap_update ?y (heapToEnv \<Gamma> (\<lambda>e. \<lbrakk> e \<rbrakk>\<^bsub>fmap_bottom (fdom ?y \<union> fst ` set \<Gamma>)\<^esub>))\<^esub>)) x') "
+              
+              sorry
+            also have "... \<sqsubseteq> the (lookup (fmap_update ?y (heapToEnv \<Gamma> (\<lambda>e. \<lbrakk> e \<rbrakk>\<^bsub>fmap_update ?y (heapToEnv \<Gamma> (\<lambda>e. \<lbrakk> e \<rbrakk>\<^bsub>fmap_bottom (fdom ?y \<union> fst ` set \<Gamma>)\<^esub>))\<^esub>))) x')"
+              using `x' \<in> fst \` set \<Gamma>` by simp
+            also have "... = the (lookup (iterate (Suc 1) (\<Lambda> \<rho>'. fmap_update ?y (heapToEnv \<Gamma> (\<lambda>e. \<lbrakk> e \<rbrakk>\<^bsub>\<rho>'\<^esub>)))\<cdot>(fmap_bottom (fdom ?y \<union> fst ` set \<Gamma>))) x')"
+                (is "_ = the (lookup ?rhs _)")
+              by simp
+            also
+            have "?rhs \<sqsubseteq> \<lbrace>\<Gamma>\<rbrace>?y"
+              unfolding HSem_def'''
+              by (rule iterate_below_fix[of _ _ "Suc 1"], simp)
+            have "?rhs \<sqsubseteq> \<lbrace>\<Gamma>\<rbrace>?y"
+              unfolding HSem_def'''
+              by (rule iterate_below_fix[of _ _ "Suc 1"], simp)
+            hence "the (lookup ?rhs x') \<sqsubseteq> the (lookup ((fmap_restr (fst ` set \<Gamma>) (\<lbrace>\<Gamma>\<rbrace>?y))) x')"
+              apply (subst lookup_fmap_restr[OF _ `x' \<in> fst \` set \<Gamma>`])
+              apply auto[1]              
+              by (rule fmap_belowE)
+            finally
+            have "the (lookup (heapToEnv \<Gamma> (\<lambda>e. \<lbrakk> e \<rbrakk>\<^bsub>?y\<^esub>)) x') \<sqsubseteq> the (lookup ((fmap_restr (fst ` set \<Gamma>) (\<lbrace>\<Gamma>\<rbrace>?y))) x')".
+
+            have "fmap_update ?y (heapToEnv \<Gamma> (\<lambda>e. \<lbrakk> e \<rbrakk>\<^bsub>?y\<^esub>)) \<sqsubseteq> \<lbrace>\<Gamma>\<rbrace>?y"
+              thm fix1_ind
+              apply (rule fix1_ind[OF _ _ `?x0 \<sqsubseteq> ?R\<cdot>?x0`]) back back back back back
+              apply auto[1]
+
+              (* Base case *)
+              apply (subst (2) HSem_unroll)
+              apply (rule cont2monofunE) back back              
+              apply auto[1]
+              apply (rule fmap_bottom_below)
+              apply auto[1]
+
+              apply (subst (3) HSem_unroll)
+              apply simp
+              apply (rule cont2monofunE) back back
+              apply auto[1]
+              apply (erule rev_below_trans)
+              
+
+
+
+
+            have "the (lookup (heapToEnv \<Gamma> (\<lambda>e. \<lbrakk> e \<rbrakk>\<^bsub>?y\<^esub>)) x') \<sqsubseteq> the (lookup ((fmap_restr (fst ` set \<Gamma>) (\<lbrace>\<Gamma>\<rbrace>?y))) x')"
+              using  `x' \<in> fst \` set \<Gamma>`  `x' \<noteq> x`
+              apply (subst (2) HSem_def'')
+              apply simp
+              apply (subst lookup_fmap_restr[OF _ `x' \<in> fst \` set \<Gamma>`])
+              apply simp
+              apply (rule fix1_ind) back
+              defer
+              apply (subst fix_eq)
+              apply auto[1]
+              apply simp
+              apply (rule cont2monofunE) back back back
+              apply simp
+              apply (rule fmap_bottom_below)
+              apply auto[1]
+              apply (rule fmap_bottom_below)
+              apply auto[1]
+              
+              apply (subst fix_eq) apply auto[1]
+              
+              apply simp
+              apply (rule cont2monofunE) back back back 
+              apply simp
+              apply auto[1]
+              thm fmap_belowE[OF below_trans[OF _ iterate_below_fix[of _ _ "1", simplified]]]
+              apply (rule  fmap_belowE[OF below_trans[OF _ iterate_below_fix[of _ _ "1", simplified]]])
+              apply simp
+              find_theorems "fix"
+              apply (subst (3) fix_eq)
+              apply auto[1]
+              apply simp
+              sorry
+            have "the (lookup (heapToEnv \<Gamma> (\<lambda>e. \<lbrakk> e \<rbrakk>\<^bsub>?y\<^esub>)) x') \<sqsubseteq> the (lookup ?y x')" sorry
+            *)
+            have "the (lookup (heapToEnv \<Gamma> (\<lambda>e. \<lbrakk> e \<rbrakk>\<^bsub>?y\<^esub>)) x') \<sqsubseteq> the (lookup (?R \<cdot> ?y) x')" sorry
+          }
+          ultimately
+          show ?thesis using `x' \<noteq> x` by simp
+        next
+        case False with F1 show ?thesis by auto
+        qed
+      qed
+    qed
+    thus "?L\<cdot>?y \<sqsubseteq> ?y"
+      apply (subst (asm)  fix_eq[symmetric])
+      by (auto intro!:fmap_bottom_below)
+  qed
+next
+  show "fix1 ?x0 ?R \<sqsubseteq> fix1 ?x0 ?L"
+  proof (rule fix_least_below[OF `?x0 \<sqsubseteq> ?R\<cdot>?x0`])
+    show "?x0 \<sqsubseteq> fix1 ?x0 ?L" by (rule start_below_fix1[OF `?x0 \<sqsubseteq> ?L\<cdot>?x0`])
+  next
+    show "?R\<cdot>(fix1 ?x0 ?L) \<sqsubseteq> fix1 ?x0 ?L"
+    proof (rule fmap_belowI')
+      show "fdom (?R\<cdot>(fix1 ?x0 ?L)) = fdom (fix1 ?x0 ?L)" by auto
+    next
+      fix x'
+      assume "x' \<in> fdom (?R\<cdot>(fix1 ?x0 ?L))" and "x' \<in> fdom (fix1 ?x0 ?L)"
+      show "the (lookup (?R\<cdot>(fix1 ?x0 ?L)) x') \<sqsubseteq> the (lookup ((fix1 ?x0 ?L)) x')"
+      proof (cases "x' = x")
+      case True thus ?thesis  by (subst (2) fix_eq, auto)
+      next
+      case False note F1 = this
+        show ?thesis
+        proof (cases "x' \<in> fst ` set \<Gamma>")
+        case True
+          from `x \<notin> fst \` set \<Gamma>`
+          have "fmap_update (fix1 ?x0 ?L) (heapToEnv \<Gamma> (\<lambda>e. \<lbrakk> e \<rbrakk>\<^bsub>(fix1 ?x0 ?L)\<^esub>)) \<sqsubseteq> (fix1 ?x0 ?L)"
+            apply -
+            apply (rule fmap_update_belowI[OF _ _ below_refl])
+            apply auto[1]
+            apply (subst (2) fix_eq)
+            apply auto[1]
+            apply (subst beta_cfun)
+            apply auto[1]
+            apply (subgoal_tac "a \<noteq> x")
+            apply auto
+            done
+          hence "fix1 (fmap_bottom (fdom ((fix1 ?x0 ?L)) \<union> fst ` set ((x, e) # \<Gamma>))) (\<Lambda> y. fmap_update (fix1 ?x0 ?L) (heapToEnv \<Gamma> (\<lambda>e. \<lbrakk> e \<rbrakk>\<^bsub>y\<^esub>))) \<sqsubseteq> (fix1 ?x0 ?L)"
+            apply -
+            apply (rule fix_least_below)
+            apply (rule fmap_bottom_below)
+            apply auto[1]
+            apply (rule fmap_bottom_below)
+            apply auto
+            done
+          hence "(\<lbrace>\<Gamma>\<rbrace>(fix1 ?x0 ?L)) \<sqsubseteq> (fix1 ?x0 ?L)"
+            unfolding HSem_def'''
+            by auto
+          with True F1
+          show ?thesis
+            apply simp
+            apply (subst lookup_fmap_restr)
+            apply auto[2]
+            apply (erule fmap_belowE)
+            done
+       next
+       case False note F2 = this
+         with F1 show ?thesis 
+          apply (subst (2) fix_eq)
+          apply auto[1]
+          apply simp
+          done
+       qed
+     qed
+   qed
+  qed
+}
+qed
+*)
+
+(*
+lemma HSem_fdom[simp]:"fdom (\<lbrace>\<Gamma>\<rbrace>\<rho>) = fst ` set \<Gamma> \<union> fdom \<rho>"
+  by (subst HSem_def', auto)
+*)
+
+(*
+lemma the_lookup_HSem_other:
+  "y \<notin> fst ` set h \<Longrightarrow> the (lookup (\<lbrace>h\<rbrace>\<rho>) y) = the (lookup \<rho> y)"
+  unfolding HSem_def'
+  by (induct rule:fix1_ind, auto)
+*)
+
+lemmas HSem_fresh[simp] = eqvt_fresh_cong2[of HSem, OF HSem_eqvt]
+ and   asToHeap_fresh[simp] = eqvt_fresh_cong1[of asToHeap, OF asToHeap.eqvt]
+ and   fresh_fmap_upd[simp] = eqvt_fresh_cong3[of fmap_upd, OF fmap_upd_eqvt]
+
+lemma fresh_fmap_upd'[simp]: "\<lbrakk> atom a \<sharp> \<rho>; atom x \<sharp> a ; atom a \<sharp> v \<rbrakk> \<Longrightarrow> atom a \<sharp> \<rho>(x f\<mapsto> v)"
+  by (metis fresh_at_base(2) fresh_fmap_upd)
+  
+lemma[simp]: "S \<sharp>* (\<rho>::Env) \<Longrightarrow> S \<sharp>* x  \<Longrightarrow> S \<sharp>* \<rho>(x f\<mapsto> the (lookup \<rho> y))"
+  apply (auto simp add: fresh_star_def) 
+  apply (rule fresh_fmap_upd)
+  apply (auto simp add: pure_fresh)
+  done    
+
+lemma ESem_subst: "x \<noteq> y \<Longrightarrow> atom x \<sharp> \<rho> \<Longrightarrow> \<lbrakk> e \<rbrakk>\<^bsub>\<rho>(x f\<mapsto> \<lbrakk>Var y\<rbrakk>\<^bsub>\<rho>\<^esub>)\<^esub> = \<lbrakk> e[x::= y] \<rbrakk>\<^bsub>\<rho>\<^esub>"
+  and 
+  "x \<noteq> y \<Longrightarrow> atom x \<sharp> \<rho> \<Longrightarrow> heapToEnv (asToHeap as) (\<lambda>e. \<lbrakk> e \<rbrakk>\<^bsub>\<rho>(x f\<mapsto> the (lookup \<rho> y))\<^esub>)
+                    = heapToEnv (asToHeap as[x::a=y]) (\<lambda>e. \<lbrakk> e \<rbrakk>\<^bsub>\<rho>\<^esub>) "
+proof (nominal_induct e and as  avoiding: \<rho> x y rule:exp_assn.strong_induct)
+case (Var var \<rho> x y) thus ?case by auto
+next
+case (App exp var \<rho> x y) thus ?case by auto
+next
+case (Let as exp \<rho> x y)
+  from `set (bn as) \<sharp>* x` `set (bn as) \<sharp>* y` 
+  have "x \<notin> assn_vars as " "y \<notin> assn_vars as "
+    by (induct as rule: assn_vars.induct, auto simp add: exp_assn.bn_defs fresh_star_insert)
+  hence [simp]:"assn_vars (as[x::a=y]) = assn_vars as" 
+     by (induct as rule: assn_vars.induct, auto)
+
+  have "\<lbrace>asToHeap as\<rbrace>\<rho>(x f\<mapsto> the (lookup \<rho> y))  = fmap_update (\<rho>(x f\<mapsto> the (lookup \<rho> y)))
+     (fix1 (fmap_bottom (fst ` set (asToHeap as)))
+       (\<Lambda> \<rho>'a. (heapToEnv (asToHeap as)(\<lambda>e. \<lbrakk> e \<rbrakk>\<^bsub>fmap_update (\<rho>(x f\<mapsto> the (lookup \<rho> y))) \<rho>'a\<^esub>))))"
+    apply (subst HSem_def') .. also
+  have "... = fmap_update (\<rho>(x f\<mapsto> the (lookup \<rho> y)))
+     (fix1 (fmap_bottom (fst ` set (asToHeap as)))
+       (\<Lambda> \<rho>'a. (heapToEnv (asToHeap as)(\<lambda>e. \<lbrakk> e \<rbrakk>\<^bsub>(fmap_update \<rho> \<rho>'a)(x f\<mapsto> the (lookup (fmap_update \<rho> \<rho>'a) y))\<^esub>))))"
+    apply (rule arg_cong)back
+    using `x \<notin> _`  `y \<notin> _`
+    apply (auto intro: fix1_cong simp add: fmap_update_upd_swap)
+    done also
+  have "... = fmap_update (\<rho>(x f\<mapsto> the (lookup \<rho> y)))
+     (fix1 (fmap_bottom (fst ` set (asToHeap as)))
+       (\<Lambda> \<rho>'a. (heapToEnv (asToHeap (as[x ::a= y]))(\<lambda>e. \<lbrakk> e \<rbrakk>\<^bsub>(fmap_update \<rho> \<rho>'a)\<^esub>))))"
+      apply (rule arg_cong)back
+      apply (rule fix1_cong)
+      apply auto[2]
+      apply simp
+      apply (subst `_ \<Longrightarrow> _ \<Longrightarrow> heapToEnv _ _ = _`[OF `x \<noteq> y`])
+      using `atom x \<sharp> \<rho>` `x \<notin> assn_vars as`
+      apply (auto simp add:sharp_Env)
+    done also
+  have "... = (fmap_update \<rho>
+     (fix1 (fmap_bottom (fst ` set (asToHeap (as[x ::a= y]))))
+       (\<Lambda> \<rho>'a. (heapToEnv (asToHeap (as[x ::a= y]))(\<lambda>e. \<lbrakk> e \<rbrakk>\<^bsub>(fmap_update \<rho> \<rho>'a)\<^esub>)))))(x f\<mapsto> the (lookup \<rho> y))"
+       using `x \<notin> assn_vars as` by (auto simp add: fmap_update_upd_swap) also
+  have "... = (\<lbrace> asToHeap as[x ::a= y]\<rbrace>\<rho>) (x f\<mapsto> the (lookup \<rho> y))"
+    by (subst HSem_def', simp) also
+  have "... = (\<lbrace> asToHeap as[x ::a= y]\<rbrace>\<rho>) (x f\<mapsto> the (lookup (\<lbrace> asToHeap as[x ::a= y]\<rbrace>\<rho>) y))"
+    using `y \<notin> assn_vars as`
+    by (auto simp add: the_lookup_HSem_other)
+  finally
+  have "\<lbrace>asToHeap as\<rbrace>(\<rho>(x f\<mapsto> the (lookup \<rho> y))) = (\<lbrace>asToHeap (as[x ::a= y])\<rbrace>\<rho>)(x f\<mapsto> the (lookup (\<lbrace>asToHeap (as[x ::a= y])\<rbrace>\<rho>) y))" .
+  with Let
+  show ?case
+  by (auto simp add: fresh_star_Pair fresh_at_base)
+next
+case (Lam var exp \<rho> x' y) thus ?case
+  apply (auto simp add: fresh_star_Pair pure_fresh)
+  apply (subst fmap_upd_twist)
+  apply (auto)[1]
+  apply (rule cfun_eqI) 
+  apply (erule_tac x = "x'" in meta_allE)
+  apply (erule_tac x = "y" in meta_allE)
+  apply (erule_tac x = "\<rho>(var f\<mapsto> x)" in meta_allE)
+  apply (auto simp add: pure_fresh fresh_at_base)[1]
+  done
+next
+case (ANil \<rho> x y) thus ?case by auto
+next
+case(ACons var exp as \<rho> x y)  thus ?case by auto
+qed
+
+
+end
